

$$Q-1(a) \quad |+\rangle = \frac{1}{\sqrt{2}} (|0\rangle + |1\rangle)$$

$$= \frac{1}{\sqrt{2}} \left(\begin{pmatrix} 1 \\ 0 \end{pmatrix} + \begin{pmatrix} 0 \\ 1 \end{pmatrix} \right) = \frac{1}{\sqrt{2}} \begin{pmatrix} 1 \\ 1 \end{pmatrix}$$

~~Q-1(b)~~
$$|-\rangle = \frac{1}{\sqrt{2}} (|0\rangle - |1\rangle)$$

$$= \frac{1}{\sqrt{2}} \left(\begin{pmatrix} 1 \\ 0 \end{pmatrix} - \begin{pmatrix} 0 \\ 1 \end{pmatrix} \right) = \frac{1}{\sqrt{2}} \begin{pmatrix} 1 \\ -1 \end{pmatrix}$$

$$(b) \quad |+\rangle = \frac{1}{\sqrt{2}} \begin{Bmatrix} |0\rangle + \frac{1}{\sqrt{2}} |1\rangle \end{Bmatrix} \quad -\textcircled{1}$$

$$|-\rangle = \frac{1}{\sqrt{2}} |0\rangle - \frac{1}{\sqrt{2}} |1\rangle \quad -\textcircled{2}$$

$$|0\rangle = \frac{1}{\sqrt{2}} (|+\rangle + |-\rangle) \quad \text{Adding } \textcircled{1} \text{ \& } \textcircled{2}$$

$$|1\rangle = \frac{1}{\sqrt{2}} (|+\rangle - |-\rangle) \quad \text{Subtracting } \textcircled{2} \text{ from } \textcircled{1}$$

~~(c) $|+\rangle = \frac{1}{\sqrt{2}} \begin{pmatrix} \frac{1}{\sqrt{3}} \\ -i\sqrt{\frac{2}{3}} \end{pmatrix}$~~

$$= \begin{pmatrix} \frac{1}{\sqrt{3}} \\ 0 \end{pmatrix} + \begin{pmatrix} 0 \\ -i\sqrt{\frac{2}{3}} \end{pmatrix} = \begin{pmatrix} \frac{1}{\sqrt{3}} \\ 0 \end{pmatrix} + -i\sqrt{\frac{2}{3}} \begin{pmatrix} 1 \\ 0 \end{pmatrix}$$

$$= \frac{1}{\sqrt{3}} |0\rangle - i\sqrt{\frac{2}{3}} |1\rangle$$

(d) From (b)

$$|+\rangle = \frac{1}{\sqrt{3}} \left(\frac{1}{\sqrt{2}} (|+\rangle + |-\rangle) \right) - i\sqrt{\frac{2}{3}} \cdot \frac{1}{\sqrt{2}} (|+\rangle - |-\rangle)$$

$$= \frac{1}{\sqrt{3}} \cdot \frac{1}{\sqrt{2}} \begin{Bmatrix} |+\rangle + \frac{1}{\sqrt{3}} \cdot \frac{1}{\sqrt{2}} |-\rangle - \frac{1}{\sqrt{3}} |+\rangle + \frac{i}{\sqrt{3}} |-\rangle \end{Bmatrix}$$

$$= \frac{1}{\sqrt{3}} \left(\frac{1}{\sqrt{2}} - i \right) |+\rangle + \frac{1}{\sqrt{3}} \left(\frac{1}{\sqrt{2}} + i \right) |-\rangle$$

$$Q-2(a) \quad |+\rangle = \frac{1}{\sqrt{2}} (|0\rangle + |1\rangle)$$

$$|-\rangle = \frac{1}{\sqrt{2}} (|0\rangle - |1\rangle)$$

$$|+\rangle \otimes |-\rangle = \left(\frac{1}{\sqrt{2}} |0\rangle + \frac{1}{\sqrt{2}} |1\rangle \right) \otimes \left(\frac{1}{\sqrt{2}} |0\rangle - \frac{1}{\sqrt{2}} |1\rangle \right)$$

~~$$= \frac{1}{2} |0\rangle \otimes |0\rangle - \frac{1}{2} |0\rangle \otimes |1\rangle + \frac{1}{2} |1\rangle \otimes |0\rangle - \frac{1}{2} |1\rangle \otimes |1\rangle$$~~

$$= \frac{1}{2} |0\rangle \otimes |0\rangle - \frac{1}{2} |0\rangle \otimes |1\rangle + \frac{1}{2} |1\rangle \otimes |0\rangle - \frac{1}{2} |1\rangle \otimes |1\rangle$$

$$= \frac{1}{2} |00\rangle - \frac{1}{2} |01\rangle + \frac{1}{2} |10\rangle - \frac{1}{2} |11\rangle$$

$$(b) \text{ since, } |00\rangle = \begin{pmatrix} 1 \\ 0 \\ 0 \end{pmatrix} \quad |01\rangle = \begin{pmatrix} 0 \\ 1 \\ 0 \end{pmatrix} \quad |10\rangle = \begin{pmatrix} 0 \\ 0 \\ 1 \end{pmatrix} \quad |11\rangle = \begin{pmatrix} 0 \\ 0 \\ 1 \end{pmatrix}$$

Substituting these vectors in (a)

~~$$|+\rangle \otimes |-\rangle = \frac{1}{2} \begin{pmatrix} 1 \\ 0 \\ 0 \end{pmatrix} - \frac{1}{2} \begin{pmatrix} 0 \\ 1 \\ 0 \end{pmatrix} + \frac{1}{2} \begin{pmatrix} 0 \\ 0 \\ 1 \end{pmatrix} - \frac{1}{2} \begin{pmatrix} 0 \\ 0 \\ 1 \end{pmatrix}$$~~

$$|+\rangle \otimes |-\rangle = \frac{1}{2} \begin{pmatrix} 1 \\ 0 \\ 0 \end{pmatrix} - \frac{1}{2} \begin{pmatrix} 0 \\ 1 \\ 0 \end{pmatrix} + \frac{1}{2} \begin{pmatrix} 0 \\ 0 \\ 1 \end{pmatrix} - \frac{1}{2} \begin{pmatrix} 0 \\ 0 \\ 1 \end{pmatrix}$$

$$= \frac{1}{2} \begin{pmatrix} 1 \\ -1 \\ 0 \end{pmatrix}$$

$$(c) |N\rangle = \begin{pmatrix} 1/\sqrt{2} \\ i/\sqrt{2} \\ 0 \end{pmatrix} = \frac{1}{\sqrt{2}} \begin{pmatrix} 1 \\ 0 \\ 0 \end{pmatrix} + \frac{i}{2\sqrt{2}} \begin{pmatrix} 0 \\ 1 \\ 0 \end{pmatrix} + \frac{1}{2\sqrt{2}} \begin{pmatrix} 0 \\ 0 \\ 1 \end{pmatrix}$$

$$= \frac{1}{\sqrt{2}} |00\rangle + \frac{i}{2\sqrt{2}} |10\rangle + \frac{1}{2\sqrt{2}} |11\rangle$$

$$8-3 \text{ (a) } |N\rangle = (X \otimes H) (|0\rangle \otimes |1\rangle)$$

$$= X |0\rangle \otimes H |1\rangle$$

$$\text{Now, } X |0\rangle = |1\rangle$$

$$\begin{aligned} H |1\rangle &= H \cdot H |0\rangle \quad (\text{since } |1\rangle = H \cdot |0\rangle) \\ &= H^2 |0\rangle = |0\rangle \quad (\text{since } H \text{ is unitary}) \end{aligned}$$

$$\therefore |N\rangle = |1\rangle \otimes |0\rangle = |10\rangle$$

$$(b) X \otimes H$$

$$X \otimes H |00\rangle = |11\rangle$$

$$X \otimes H |01\rangle = |10\rangle$$

$$X \otimes H |10\rangle = |01\rangle$$

$$X \otimes H |11\rangle = |00\rangle$$

Using these eq^s, the matrix $X \otimes H$ will be

$$X \otimes H = \begin{bmatrix} 0 & 0 & 1/\sqrt{2} & 1/\sqrt{2} \\ 0 & 0 & 1/\sqrt{2} & -1/\sqrt{2} \\ 1/\sqrt{2} & 1/\sqrt{2} & 0 & 0 \\ 1/\sqrt{2} & -1/\sqrt{2} & 0 & 0 \end{bmatrix}$$

Since the matrix is a linear map of basis vectors.

$$(c) |0\rangle \otimes |1\rangle = \begin{bmatrix} 1 \\ 0 \end{bmatrix} \otimes \begin{bmatrix} 1/\sqrt{2} \\ 1/\sqrt{2} \end{bmatrix}$$

$$= \begin{bmatrix} 1 \cdot 1/\sqrt{2} \\ 1 \cdot 1/\sqrt{2} \\ 0 \cdot 1/\sqrt{2} \\ 0 \cdot 1/\sqrt{2} \end{bmatrix} = \begin{bmatrix} 1/\sqrt{2} \\ 1/\sqrt{2} \\ 0 \\ 0 \end{bmatrix}$$

$$(d) |1\rangle \otimes |0\rangle = \begin{bmatrix} 1/\sqrt{2} \\ -1/\sqrt{2} \end{bmatrix} \otimes \begin{bmatrix} 1 \\ 0 \end{bmatrix} = \begin{bmatrix} 1/\sqrt{2} \cdot 1 \\ -1/\sqrt{2} \cdot 1 \\ 1/\sqrt{2} \cdot 0 \\ -1/\sqrt{2} \cdot 0 \end{bmatrix} = \begin{bmatrix} 1/\sqrt{2} \\ -1/\sqrt{2} \\ 0 \\ 0 \end{bmatrix}$$

$$= \begin{bmatrix} 1/\sqrt{2} \\ 0 \\ -1/\sqrt{2} \\ 0 \end{bmatrix}$$

Q-4 (a) since A is a linear map.

$$A = \begin{bmatrix} 0 & 0 & 0 & 1 \\ 0 & 0 & 1 & 0 \\ 1 & 0 & 0 & 0 \\ 0 & 1 & 0 & 0 \end{bmatrix}$$

(b) For A to be unitary, A^T should be A^{-1}

$$A^T = \begin{bmatrix} 0 & 0 & 1 & 0 \\ 0 & 0 & 0 & 1 \\ 0 & 1 & 0 & 0 \\ 1 & 0 & 0 & 0 \end{bmatrix}$$

$$A \cdot A^T = \begin{bmatrix} 0 & 0 & 0 & 1 \\ 0 & 0 & 0 & 1 \\ 0 & 0 & 1 & 0 \\ 1 & 0 & 0 & 0 \end{bmatrix} \cdot \begin{bmatrix} 0 & 0 & 1 & 0 \\ 0 & 0 & 0 & 1 \\ 0 & 1 & 0 & 0 \\ 1 & 0 & 0 & 0 \end{bmatrix} = \begin{bmatrix} 1 & 0 & 0 & 0 \\ 0 & 1 & 0 & 0 \\ 0 & 0 & 1 & 0 \\ 0 & 0 & 0 & 1 \end{bmatrix} = I$$

Hence, A is unitary.

(c) since A is unitary A^{-1} is A^T

$$A^{-1} = \begin{bmatrix} 0 & 0 & 1 & 0 \\ 0 & 0 & 0 & 1 \\ 0 & 1 & 0 & 0 \\ 1 & 0 & 0 & 0 \end{bmatrix}$$

$$A^{-1} |00\rangle = \begin{bmatrix} 0 & 0 & 1 & 0 \\ 0 & 0 & 0 & 1 \\ 0 & 1 & 0 & 0 \\ 1 & 0 & 0 & 0 \end{bmatrix} \begin{bmatrix} 1 \\ 0 \\ 0 \\ 0 \end{bmatrix} = \begin{bmatrix} 0 \\ 0 \\ 0 \\ 1 \end{bmatrix} = |11\rangle$$

$$A^{-1} |01\rangle = \begin{bmatrix} 0 & 0 & 1 & 0 \\ 0 & 0 & 0 & 1 \\ 0 & 1 & 0 & 0 \\ 1 & 0 & 0 & 0 \end{bmatrix} \begin{bmatrix} 0 \\ 1 \\ 0 \\ 0 \end{bmatrix} = \begin{bmatrix} 0 \\ 1 \\ 0 \\ 0 \end{bmatrix} = |00\rangle$$

$$A^{-1} |10\rangle = \begin{bmatrix} 0 & 0 & 1 & 0 \\ 0 & 0 & 0 & 1 \\ 0 & 1 & 0 & 0 \\ 1 & 0 & 0 & 0 \end{bmatrix} \begin{bmatrix} 0 \\ 0 \\ 1 \\ 0 \end{bmatrix} = \begin{bmatrix} 1 \\ 0 \\ 0 \\ 0 \end{bmatrix} = |10\rangle$$

$$A^{-1} |11\rangle = \begin{bmatrix} 0 & 0 & 1 & 0 \\ 0 & 0 & 0 & 1 \\ 0 & 1 & 0 & 0 \\ 1 & 0 & 0 & 0 \end{bmatrix} \begin{bmatrix} 0 \\ 0 \\ 0 \\ 1 \end{bmatrix} = \begin{bmatrix} 0 \\ 1 \\ 0 \\ 0 \end{bmatrix} = |01\rangle$$

$$8-5(a) \quad |Y_0\rangle = |000\rangle$$

$$|Y_1\rangle = \frac{1}{\sqrt{2}} |100\rangle$$

$$= \left(\frac{1}{\sqrt{2}} |0\rangle + \frac{1}{\sqrt{2}} |1\rangle \right) \frac{1}{\sqrt{2}} |00\rangle = \frac{1}{\sqrt{2}} |000\rangle + \frac{1}{\sqrt{2}} |100\rangle$$

$$|Y_2\rangle = \frac{1}{\sqrt{2}} |100\rangle + \frac{1}{\sqrt{2}} |120\rangle$$

$$|Y_3\rangle = \frac{1}{\sqrt{2}} |100\rangle + \frac{1}{\sqrt{2}} |111\rangle$$

$$8(b) \quad |Y_3\rangle = \frac{1}{\sqrt{2}} |100\rangle + \frac{1}{\sqrt{2}} |111\rangle$$

$$\text{Now, } |0\rangle = \frac{1}{\sqrt{2}} (|+\rangle + |-\rangle) \quad |1\rangle = \frac{1}{\sqrt{2}} (|+\rangle - |-\rangle)$$

Substituting $\frac{1}{\sqrt{2}} |+\rangle$ by a and $\frac{1}{\sqrt{2}} |-\rangle$ by b

$$|Y_3\rangle = \frac{1}{\sqrt{2}} [(a+b) \cdot (a+b) \cdot (a+b) + (a-b) \cdot (a-b) \cdot (a-b)]$$

$$= \frac{1}{\sqrt{2}} [(a \cdot a + a \cdot b + \cancel{a \cdot a} + b \cdot a + b \cdot b) (a+b) + (a \cdot a - a \cdot b - b \cdot a + b \cdot b) (a-b)]$$

$$= \frac{1}{\sqrt{2}} [a \cdot a \cdot a + a \cdot a \cdot b + a \cdot b \cdot a + b \cdot a \cdot a + b \cdot a \cdot b + b \cdot b \cdot a + b \cdot b \cdot a - a \cdot a \cdot b - a \cdot b \cdot a - b \cdot a \cdot a - b \cdot a \cdot b - b \cdot b \cdot a - b \cdot b \cdot b]$$

$$= \frac{1}{\sqrt{2}} [2 \cdot a \cdot a \cdot a + 2 \cdot a \cdot b \cdot b + 2 \cdot b \cdot a \cdot b + 2 \cdot b \cdot b \cdot a]$$

$$= \frac{1}{\sqrt{2}} \left[\frac{2 \cdot 1}{2\sqrt{2}} |++\rangle + \frac{2 \cdot 1}{2\sqrt{2}} |+-\rangle + \frac{2 \cdot 1}{2\sqrt{2}} |-+\rangle + \frac{2 \cdot 1}{2\sqrt{2}} |--\rangle \right]$$

$$= \frac{1}{2} (|++\rangle + |+-\rangle + |-+\rangle + |--\rangle)$$

$$(c) \quad |Y_3\rangle = \frac{1}{\sqrt{2}} |100\rangle + \frac{1}{\sqrt{2}} |111\rangle$$

$$\rho(|100\rangle) = \left(\frac{1}{\sqrt{2}} \right)^2 = \frac{1}{2}$$

$$\rho(|111\rangle) = \left(\frac{1}{\sqrt{2}} \right)^2 = \frac{1}{2}$$